State.thy
@@ -1,0 +1,461 @@
+theory State
+  imports Main
+begin
+
+chapter \<open>Abstract State\<close>
+
+text \<open>
+To ensure the logic is sufficiently abstract,
+we make no assumptions about its structure and represent it as a single type variable.
+Therefore, rules that manipulate the state, such as removal of auxiliary variables
+and local state require operators over the state to express the necessary transformations.
+\<close>
+
+type_synonym ('b) pred = "('b) set"
+type_synonym ('b) rpred = "('b) rel"
+
+section \<open>Definitions\<close>
+
+text \<open>Stability of a predicate across an environment step\<close>
+definition stable :: "('b) rpred \<Rightarrow> ('b) pred \<Rightarrow> bool"
+  where "stable R P \<equiv> \<forall>m m'. m \<in> P \<longrightarrow> (m,m') \<in> R \<longrightarrow> m' \<in> P"
+
+text \<open>Weakest precondition for a pre-condition and post-relation\<close>
+definition wp :: "'b pred \<Rightarrow> 'b rpred \<Rightarrow> 'b pred \<Rightarrow> 'b pred"
+  where "wp pre post Q \<equiv> pre \<inter> {m. (\<forall>m'. (m,m') \<in> post \<longrightarrow> m' \<in> Q)}"
+
+text \<open>Guarantee check for a pre-condition and post-relation\<close>
+definition guar :: "'b pred \<Rightarrow> 'b rpred \<Rightarrow> 'b rpred \<Rightarrow> bool"
+  where "guar pre post G \<equiv> {(m,m'). m \<in> pre \<and> (m,m') \<in> post} \<subseteq> G"
+
+text \<open>Shorthand for the weakest-precondition of an environment step\<close>
+abbreviation wp\<^sub>e :: "'b rpred \<Rightarrow> 'b pred \<Rightarrow> 'b pred"
+  where "wp\<^sub>e R Q \<equiv> wp UNIV (R\<^sup>* ) Q"
+
+section \<open>Stability Properties\<close>
+
+lemma stable_conseqI [intro]:
+  assumes "stable R' P" "R \<subseteq> R'" 
+  shows "stable R P"
+  using assms rtrancl_mono unfolding stable_def by blast
+
+lemma stable_conjI [intro]:
+  assumes "stable R P" "stable R' P'"
+  shows "stable (R \<inter> R') (P \<inter> P')"
+  using assms by (auto simp: stable_def)
+
+lemma stable_transitive:
+  assumes "(m,m') \<in> R\<^sup>*" "m \<in> P" "stable R P"
+  shows "m' \<in> P"
+  using assms by (induct rule: rtrancl.induct) (auto simp: stable_def)
+
+lemma stable_wpI:
+  "stable R P \<Longrightarrow> P \<subseteq> wp UNIV (R\<^sup>*) P"
+  unfolding wp_def using stable_transitive by fast
+
+lemma stable_falseI [intro]:
+  "stable R {}"
+  by (auto simp: stable_def)
+
+section \<open>Guarantee Properties\<close>
+
+lemma guar_conseqI [intro]:
+  assumes "guar pre post G" "G \<subseteq>  G'"
+  shows "guar pre post G'"
+  using assms by (auto simp: guar_def)
+
+section \<open>Thread-Local State\<close>
+
+text \<open>
+To support thread-local state, we require an operation capable of merging two states, such
+that the global component from the first is merged with the local component of the second.
+We refer to this operation as op throughout the definitions.
+\<close>
+
+type_synonym 'b merge = "'b \<Rightarrow> 'b \<Rightarrow> 'b"
+
+text \<open>Collect all states where their combination with the local state of l satisfies P\<close>
+definition thr\<^sub>P :: "'b merge \<Rightarrow> 'b \<Rightarrow> 'b pred \<Rightarrow> 'b pred"
+  where "thr\<^sub>P op l P \<equiv> {m. op m l \<in> P}"
+
+text \<open>Collect all states where some local state satisfies Q\<close>
+definition thr\<^sub>Q :: "'b merge \<Rightarrow> 'b pred \<Rightarrow> 'b pred"
+  where "thr\<^sub>Q op P \<equiv> {m. \<exists>l. op m l \<in> P}"
+
+text \<open>Collect all transitions in R that preserve the local state\<close>
+definition thr\<^sub>R :: "'b merge \<Rightarrow> 'b rpred \<Rightarrow> 'b rpred"
+  where "thr\<^sub>R op R \<equiv> {(m,m') |m m'. \<forall>l. (op m l,op m' l) \<in> R}"
+
+text \<open>Collect all transitions where their combinations with arbitrary local states satisfies G\<close>
+definition thr\<^sub>G :: "'b merge \<Rightarrow> 'b rpred \<Rightarrow> 'b rpred"
+  where "thr\<^sub>G op G \<equiv> {(m,m') |m m' l l'. (op m l,op m' l') \<in> G}"
+
+text \<open>Lift a local transition to a global transition given the pre and post local state\<close>
+definition thr2glb :: "'b merge \<Rightarrow> 'b \<Rightarrow> 'b \<Rightarrow> 'b rpred \<Rightarrow> 'b rpred"
+  where "thr2glb op l l' r \<equiv> {(m,m'). (op m l,op m' l') \<in> r}"
+
+text \<open>The predicate transformations preserve ordering\<close>
+lemma thr_mono:
+  "P \<subseteq> Q \<Longrightarrow> thr\<^sub>P op l P \<subseteq> thr\<^sub>P op l Q"
+  unfolding thr\<^sub>P_def by auto
+
+text \<open>The predicate transformations preserve stability\<close>
+lemma thr_stable:
+  "stable R P \<Longrightarrow> stable (thr\<^sub>R op R) (thr\<^sub>P op l P)"
+  unfolding thr\<^sub>P_def thr\<^sub>R_def stable_def by auto
+
+lemma thr_wp:
+  "P \<subseteq> wp v r M \<Longrightarrow> thr\<^sub>P op l P \<subseteq> wp (thr\<^sub>P op l v) (thr2glb op l l' r) (thr\<^sub>P op l' M)"
+  unfolding wp_def thr2glb_def thr\<^sub>P_def by auto
+
+lemma thr_guar:
+  "guar v r G \<Longrightarrow> guar (thr\<^sub>P op l v) (thr2glb op l l' r) (thr\<^sub>G op G)"
+  unfolding thr2glb_def thr\<^sub>P_def thr\<^sub>G_def guar_def by auto
+
+section \<open>Auxiliary State\<close>
+
+text \<open>
+To support auxiliary state, we require an operation capable of merging two states, such
+that the real component from the first is merged with the auxiliary component of the second.
+\<close>
+
+
+(*
+section \<open>State Expansion\<close>
+
+definition expand\<^sub>P
+  where "expand\<^sub>P m P \<equiv> \<Union> (m ` P)"
+
+definition expand\<^sub>G
+  where "expand\<^sub>G m r G \<equiv> {(c,c'). \<exists>(b,b')\<in> G. c \<in> m b \<and> c' \<in> m b' \<and> r c c'}"
+
+definition expand\<^sub>R
+  where "expand\<^sub>R m R \<equiv> {(c,c'). \<exists>(b,b')\<in> R. c \<in> m b \<and> c' \<in> m b'}"
+
+definition valid_expand
+  where "valid_expand m r \<equiv> 
+          (\<forall>b b' c. c \<in> m b' \<longrightarrow> c \<in> m b \<longrightarrow> b = b') \<and> 
+          (\<forall>a b c. r a b \<longrightarrow> a \<in> m c \<longrightarrow> b \<in> m c \<longrightarrow> a = b)"
+
+lemma expand_stable:
+  assumes "stable R P" "valid_expand m r"
+  shows "stable (expand\<^sub>R m R) (expand\<^sub>P m P)"
+  using assms unfolding stable_def valid_expand_def expand\<^sub>P_def expand\<^sub>R_def
+  by fastforce
+
+lemma expand_wp\<^sub>\<alpha>:
+  assumes "P \<subseteq> wp\<^sub>\<alpha> \<alpha> Q" "valid_expand m r"
+  assumes \<alpha>: "vc \<alpha>' = expand\<^sub>P m (vc \<alpha>)" "beh \<alpha>' = expand\<^sub>G m r (beh \<alpha>)"
+  shows "expand\<^sub>P m P \<subseteq> wp\<^sub>\<alpha> \<alpha>' (expand\<^sub>P m Q)"
+  using assms(1,2) unfolding wp_def valid_expand_def expand\<^sub>P_def expand\<^sub>G_def \<alpha>
+  by fastforce
+
+lemma expand_guar:
+  assumes "guar\<^sub>\<alpha> \<alpha> G" "valid_expand m r"
+  assumes \<alpha>: "vc \<alpha>' = expand\<^sub>P m (vc \<alpha>)" "beh \<alpha>' = expand\<^sub>G m r (beh \<alpha>)"
+  shows "guar\<^sub>\<alpha> \<alpha>' (expand\<^sub>G m r G)"
+  using assms(1,2,3) unfolding valid_expand_def expand\<^sub>G_def \<alpha> expand\<^sub>P_def guar_def
+  by blast
+
+text \<open>Expand the state of an atomic judgement\<close>
+lemma atomic_expandI [intro]:
+  assumes "R,G \<turnstile>\<^sub>A P {\<alpha> :: ('b,'a) basic} Q"
+  assumes "valid_expand m r"
+  assumes \<alpha>: "vc \<alpha>' = expand\<^sub>P m (vc \<alpha>)" "beh \<alpha>' = expand\<^sub>G m r (beh \<alpha>)" 
+  shows "expand\<^sub>R m R,expand\<^sub>G m r G \<turnstile>\<^sub>A expand\<^sub>P m P {\<alpha>' :: ('b,'c) basic} expand\<^sub>P m Q"
+  unfolding atomic_rule_def
+proof (safe)
+  show "stable (expand\<^sub>R m R) (expand\<^sub>P m P)" 
+    using assms(1,2) expand_stable unfolding atomic_rule_def by blast
+next
+  show "stable (expand\<^sub>R m R) (expand\<^sub>P m Q)" 
+    using assms(1,2) expand_stable unfolding atomic_rule_def by blast
+next
+  fix x assume "x \<in> expand\<^sub>P m P"
+  thus "x \<in> wp\<^sub>\<alpha> \<alpha>' (expand\<^sub>P m Q)"
+    using assms(1,2) \<alpha> expand_wp\<^sub>\<alpha> unfolding atomic_rule_def by blast
+next
+  show "guar\<^sub>\<alpha> \<alpha>' (expand\<^sub>G m r G)"
+    using assms(1,2) \<alpha> expand_guar unfolding atomic_rule_def by blast
+qed
+
+section \<open>Auxiliary State\<close>
+
+definition aux\<^sub>P
+  where "aux\<^sub>P r P \<equiv> {m. \<exists>m'. (m,m') \<in> r\<^sup>= \<and> m' \<in> P}"
+
+definition aux\<^sub>R
+  where "aux\<^sub>R r R \<equiv> {(m,m'). \<forall>n. (m,n) \<in> r\<^sup>= \<longrightarrow> (\<exists>n'. (m',n') \<in> r\<^sup>= \<and> (n,n') \<in> R)}"
+
+definition aux\<^sub>G
+  where "aux\<^sub>G r R \<equiv> {(m,m'). \<exists>n n'. (m,n) \<in> r\<^sup>= \<and> (m',n') \<in> r\<^sup>= \<and> (n,n') \<in> R}"
+
+lemma aux\<^sub>P_mono [intro]:
+  "P \<subseteq> Q \<Longrightarrow> aux\<^sub>P a P \<subseteq> aux\<^sub>P a Q"
+  unfolding aux\<^sub>P_def by auto
+
+lemma aux\<^sub>R_mono [intro]:
+  "P \<subseteq> Q \<Longrightarrow> aux\<^sub>R a P \<subseteq> aux\<^sub>R a Q"
+  unfolding aux\<^sub>R_def by fast
+
+lemma aux\<^sub>P_self [intro]:
+  "P \<subseteq> aux\<^sub>P r P"
+  unfolding aux\<^sub>P_def by auto
+
+lemma aux\<^sub>G_self [intro]:
+  "R \<subseteq> aux\<^sub>G r R"
+  unfolding aux\<^sub>G_def by auto
+
+lemma aux_stable [intro]:
+  assumes "stable R P" 
+  shows "stable (aux\<^sub>R r R) (aux\<^sub>P r P)"
+  unfolding stable_def aux\<^sub>R_def aux\<^sub>P_def
+proof (clarsimp, goal_cases)
+  case (1 m n p)
+  then obtain n' where a: "(p, n') \<in> r\<^sup>=" "(n, n') \<in> R" by auto
+  hence "n' \<in> P" using 1 assms by (auto simp: stable_def)
+  then show ?case using a(1) by auto
+qed
+
+abbreviation aux\<^sub>\<alpha>
+  where "aux\<^sub>\<alpha> r \<alpha> \<equiv> (tag \<alpha>, aux\<^sub>P r (vc \<alpha>), aux\<^sub>R r (beh \<alpha>))"
+
+lemma aux_wp [intro]:
+  assumes "P \<subseteq> wp\<^sub>\<alpha> \<alpha> Q"
+  shows "aux\<^sub>P r P \<subseteq> wp\<^sub>\<alpha> (aux\<^sub>\<alpha> r \<alpha>) (aux\<^sub>P r Q)"
+  unfolding wp_def aux\<^sub>P_def
+proof (clarsimp, (intro conjI; clarsimp), goal_cases)
+  case (1 n m')
+  then show ?case using assms by (auto simp: wp_def aux\<^sub>P_def)
+next
+  case (2 n m n')
+  then show ?case using assms(1) unfolding aux\<^sub>R_def wp_def by blast
+qed
+
+lemma aux_guar [intro]:
+  assumes "guar\<^sub>\<alpha> \<alpha> G" 
+  shows "guar\<^sub>\<alpha> (aux\<^sub>\<alpha> r \<alpha>) (aux\<^sub>G r G)"
+  unfolding wp_def aux\<^sub>G_def aux\<^sub>P_def aux\<^sub>R_def guar_def
+proof (clarsimp, goal_cases)
+  case (1 m m' n)
+  then obtain n' where a: "(m', n') \<in> r\<^sup>=" "(n, n') \<in> beh \<alpha>" by auto
+  hence "(n,n') \<in> G" using assms 1 by (auto simp: guar_def)
+  thus ?case using a(1) 1(3) sorry
+qed
+
+lemma atomic_auxI [intro]:
+  assumes "R,G \<turnstile>\<^sub>A P {\<alpha>} Q" 
+  shows "aux\<^sub>R r R,aux\<^sub>G r G \<turnstile>\<^sub>A aux\<^sub>P r P {aux\<^sub>\<alpha> r \<alpha>} aux\<^sub>P r Q"
+  unfolding atomic_rule_def
+proof (intro conjI)
+  show "stable (aux\<^sub>R r R) (aux\<^sub>P r P)" using assms(1) by (auto simp: atomic_rule_def)
+next
+  show "stable (aux\<^sub>R r R) (aux\<^sub>P r Q)" using assms(1) by (auto simp: atomic_rule_def)
+next
+  have "guar\<^sub>\<alpha> \<alpha> G" using assms(1) by (auto simp: atomic_rule_def)
+  thus "guar\<^sub>\<alpha> (aux\<^sub>\<alpha> r \<alpha>) (aux\<^sub>G r G)" using aux_guar by blast
+next
+  have "P \<subseteq> wp\<^sub>\<alpha> \<alpha> Q" using assms(1) by (auto simp: atomic_rule_def)
+  thus "aux\<^sub>P r P \<subseteq> wp\<^sub>\<alpha> (aux\<^sub>\<alpha> r \<alpha>) (aux\<^sub>P r Q)" using aux_wp by blast
+qed
+
+
+(*
+fun aux\<^sub>c
+  where
+    "aux\<^sub>c r Nil = Nil" |
+    "aux\<^sub>c r (Basic \<alpha>) = (Basic (aux\<^sub>\<alpha> r \<alpha>))" |
+    "aux\<^sub>c r (c\<^sub>1 ; c\<^sub>2) = (aux\<^sub>c r c\<^sub>1 ; aux\<^sub>c r c\<^sub>2)" |
+    "aux\<^sub>c r (c\<^sub>1 \<cdot> c\<^sub>2) = (aux\<^sub>c r c\<^sub>1 \<cdot> aux\<^sub>c r c\<^sub>2)" |
+    "aux\<^sub>c r (c\<^sub>1 \<sqinter> c\<^sub>2)  = (aux\<^sub>c r c\<^sub>1 \<sqinter> aux\<^sub>c r c\<^sub>2)" |
+    "aux\<^sub>c r (Loop c) = Loop (aux\<^sub>c r c)" |
+    "aux\<^sub>c r (BigChoice S\<^sub>1) = (BigChoice ((map (aux\<^sub>\<alpha> r)) ` S\<^sub>1))" |
+    "aux\<^sub>c r (Dec b m c) = (Dec b m (aux\<^sub>c r c))" |
+    "aux\<^sub>c r (c\<^sub>1 || c\<^sub>2) = (aux\<^sub>c r c\<^sub>1 || aux\<^sub>c r c\<^sub>2)"
+
+lemma aux\<^sub>c_nilE [elim!]:
+  assumes "aux\<^sub>c r c = Nil"
+  obtains "c = Nil"
+  using assms
+  by (cases "(r,c)" rule: aux\<^sub>c.cases) auto
+
+lemma aux\<^sub>c_basicE [elim!]:
+  assumes "aux\<^sub>c r c = Basic \<alpha>"
+  obtains \<beta> where "c = Basic \<beta>" "\<alpha> = aux\<^sub>\<alpha> r \<beta>"
+  using assms by (cases "(r,c)" rule: aux\<^sub>c.cases) auto
+
+lemma aux\<^sub>c_seqE [elim!]:
+  assumes "aux\<^sub>c r c = c\<^sub>1 ; c\<^sub>2"
+  obtains c\<^sub>1' c\<^sub>2' where "c = c\<^sub>1' ; c\<^sub>2'" "aux\<^sub>c r c\<^sub>1' = c\<^sub>1" "aux\<^sub>c r c\<^sub>2' = c\<^sub>2"
+  using assms by (cases "(r,c)" rule: aux\<^sub>c.cases) auto
+
+lemma aux\<^sub>c_ordE [elim!]:
+  assumes "aux\<^sub>c r c = c\<^sub>1 \<cdot> c\<^sub>2"
+  obtains c\<^sub>1' c\<^sub>2' where "c = c\<^sub>1' \<cdot> c\<^sub>2'" "aux\<^sub>c r c\<^sub>1' = c\<^sub>1" "aux\<^sub>c r c\<^sub>2' = c\<^sub>2"
+  using assms by (cases "(r,c)" rule: aux\<^sub>c.cases) auto
+
+lemma aux\<^sub>c_choiceE [elim!]:
+  assumes "aux\<^sub>c r c = c\<^sub>1 \<sqinter> c\<^sub>2"
+  obtains c\<^sub>1' c\<^sub>2' where "c = c\<^sub>1' \<sqinter> c\<^sub>2'" "aux\<^sub>c r c\<^sub>1' = c\<^sub>1" "aux\<^sub>c r c\<^sub>2' = c\<^sub>2"
+  using assms by (cases "(r,c)" rule: aux\<^sub>c.cases) auto
+
+lemma aux\<^sub>c_loopE [elim!]:
+  assumes "aux\<^sub>c r c = Loop c\<^sub>1"
+  obtains c\<^sub>1' where "c = Loop c\<^sub>1'" "aux\<^sub>c r c\<^sub>1' = c\<^sub>1" 
+  using assms by (cases "(r,c)" rule: aux\<^sub>c.cases) auto
+
+lemma aux_local [intro]:
+  assumes "local c" 
+  shows "local (aux\<^sub>c r c)"
+  using assms by (induct c rule: local.induct) auto
+*)
+
+(*
+lemma aux\<^sub>c_seqE2 [elim!]:
+  assumes "c\<^sub>1 ; c\<^sub>2 = aux\<^sub>c r c "
+  obtains c\<^sub>1' c\<^sub>2' where "c = c\<^sub>1' ; c\<^sub>2'" "aux\<^sub>c r c\<^sub>1' = c\<^sub>1" "aux\<^sub>c r c\<^sub>2' = c\<^sub>2"
+  using assms by (cases "(r,c)" rule: aux\<^sub>c.cases) auto
+
+lemma aux\<^sub>c_ordE [elim!]:
+  assumes "c\<^sub>1 \<cdot> c\<^sub>2 = aux\<^sub>c r c"
+  obtains c\<^sub>1' c\<^sub>2' where "c = c\<^sub>1' \<cdot> c\<^sub>2'" "aux\<^sub>c r c\<^sub>1' = c\<^sub>1" "aux\<^sub>c r c\<^sub>2' = c\<^sub>2"
+  using assms by (cases "(r,c)" rule: aux\<^sub>c.cases) auto
+
+lemma aux\<^sub>c_parE [elim!]:
+  assumes "c\<^sub>1 || c\<^sub>2 = aux\<^sub>c r c"
+  obtains c\<^sub>1' c\<^sub>2' where "c = c\<^sub>1' || c\<^sub>2'" "aux\<^sub>c r c\<^sub>1' = c\<^sub>1" "aux\<^sub>c r c\<^sub>2' = c\<^sub>2"
+  using assms by (cases "(r,c)" rule: aux\<^sub>c.cases) auto
+
+lemma aux\<^sub>c_choiceE [elim!]:
+  assumes "c\<^sub>1 \<sqinter> c\<^sub>2 = aux\<^sub>c r c"
+  obtains c\<^sub>1' c\<^sub>2' where "c = c\<^sub>1' \<sqinter> c\<^sub>2'" "aux\<^sub>c r c\<^sub>1' = c\<^sub>1" "aux\<^sub>c r c\<^sub>2' = c\<^sub>2"
+  using assms by (cases "(r,c)" rule: aux\<^sub>c.cases) auto
+
+lemma aux\<^sub>c_loopE [elim!]:
+  assumes "Loop c\<^sub>1 = aux\<^sub>c r c"
+  obtains c\<^sub>1' where "c = Loop c\<^sub>1'" "aux\<^sub>c r c\<^sub>1' = c\<^sub>1" 
+  using assms by (cases "(r,c)" rule: aux\<^sub>c.cases) auto
+
+lemma aux\<^sub>c_bigchoiceE [elim!]:
+  assumes "(\<Sqinter> S) = aux\<^sub>c r c"
+  obtains S' where "c = \<Sqinter> S'" "S = (map (aux\<^sub>\<alpha> r)) ` S'" 
+  using assms by (cases "(r,c)" rule: aux\<^sub>c.cases) auto
+
+lemma [simp]:
+  "seq2com (map (aux\<^sub>\<alpha> r) x) = aux\<^sub>c r (seq2com x)"
+proof (induct x)
+case Nil
+  then show ?case by auto
+next
+  case (Cons a x)
+  then show ?case  by auto
+qed
+
+lemma aux_rewriteE:
+  assumes "aux\<^sub>c r c \<leadsto> c\<^sub>a"
+  obtains c' where "c \<leadsto> c'" "aux\<^sub>c r c' = c\<^sub>a"
+  using assms
+  by (induct "aux\<^sub>c r c" c\<^sub>a arbitrary: r c) (auto; force)+
+
+lemma aux\<^sub>c_basicE [elim!]:
+  assumes "Basic \<alpha> = aux\<^sub>c r c"
+  obtains \<beta> where "c = Basic \<beta>" "\<alpha> = aux\<^sub>\<alpha> r \<beta>"
+  using assms by (cases "(r,c)" rule: aux\<^sub>c.cases) auto
+
+lemma [simp]:
+  "(aux\<^sub>\<alpha> r \<beta>)\<langle>tag x\<rangle> = aux\<^sub>\<alpha> r \<beta>\<langle>tag x\<rangle>"
+  
+  sorry
+
+lemma [simp]:
+  "(aux\<^sub>\<alpha> r \<beta>)\<llangle>aux\<^sub>c r p\<rrangle> = aux\<^sub>\<alpha> r \<beta>\<llangle>p\<rrangle>"
+  by (induct p arbitrary: \<beta>) auto
+
+lemma aux_re:
+  assumes "\<alpha>' < aux\<^sub>c r c <\<^sub>c aux\<^sub>\<alpha> r \<alpha>"
+  obtains \<beta> where "\<beta> < c <\<^sub>c \<alpha>" "\<alpha>' = aux\<^sub>\<alpha> r \<beta>"
+  using assms
+proof (induct c arbitrary: \<alpha>' \<alpha>)
+  case Nil
+  then show ?case by auto
+next
+  case (Basic x)
+  hence "tag x \<hookleftarrow> tag (\<alpha>)\<langle>tag x\<rangle>" by auto
+  moreover have "\<alpha>' = aux\<^sub>\<alpha> r \<alpha>\<langle>tag x\<rangle>" using Basic(2) by auto
+  ultimately show ?case using Basic(1) by auto
+next
+  case (Seq c1 c2)
+  then obtain \<beta> where b: "\<alpha>' < aux\<^sub>c r c1 <\<^sub>c \<beta>" "\<beta> < aux\<^sub>c r c2 <\<^sub>c aux\<^sub>\<alpha> r \<alpha>" by auto
+  show ?case 
+  proof (rule Seq(2)[OF _ b(2)])
+    fix \<beta>' assume c: "\<beta>' < c2 <\<^sub>c \<alpha>" "\<beta> = aux\<^sub>\<alpha> r \<beta>'"
+    hence a: "\<alpha>' < aux\<^sub>c r c1 <\<^sub>c aux\<^sub>\<alpha> r \<beta>'" using b by auto
+    show ?thesis apply (rule Seq(1)[OF _a]) using c(1) Seq(3) reorder_com.simps(3) by blast 
+  qed
+next
+  case (Ord c1 c2)
+  then obtain \<beta> where b: "\<alpha>' < aux\<^sub>c r c1 <\<^sub>c \<beta>" "\<beta> < aux\<^sub>c r c2 <\<^sub>c aux\<^sub>\<alpha> r \<alpha>" by auto
+  show ?case 
+  proof (rule Ord(2)[OF _ b(2)])
+    fix \<beta>' assume c: "\<beta>' < c2 <\<^sub>c \<alpha>" "\<beta> = aux\<^sub>\<alpha> r \<beta>'"
+    hence a: "\<alpha>' < aux\<^sub>c r c1 <\<^sub>c aux\<^sub>\<alpha> r \<beta>'" using b by auto
+    show ?thesis apply (rule Ord(1)[OF _a]) using c(1) Ord(3) reorder_com.simps(4) by blast 
+  qed
+qed auto
+
+lemma aux_execE:
+  assumes "aux\<^sub>c r c \<mapsto>[p,\<alpha>] c\<^sub>a"
+  obtains c' p' \<beta> where "c \<mapsto>[p',\<beta>] c'" "aux\<^sub>c r c' = c\<^sub>a" "\<alpha> = aux\<^sub>\<alpha> r \<beta>" "aux\<^sub>c r p' = p"
+  using assms
+proof (induct "aux\<^sub>c r c" p \<alpha> c\<^sub>a arbitrary: r c)
+  case (act \<alpha>)
+  then show ?case apply auto by force
+next
+  case (seq c\<^sub>1 r' \<alpha> c\<^sub>1' c\<^sub>2)
+  then show ?case apply auto by force
+next
+  case (ord c\<^sub>1 r \<alpha> c\<^sub>1' c\<^sub>2)
+  then show ?case apply auto by force
+next
+  case (ooo c\<^sub>2 r' \<alpha> c\<^sub>2' \<alpha>' c\<^sub>1)
+  then obtain c\<^sub>1' c' where s: "c = c\<^sub>1' ; c'" "c\<^sub>1 = aux\<^sub>c r c\<^sub>1'" "aux\<^sub>c r c' = c\<^sub>2" by auto
+
+  
+  show ?case 
+  proof (rule ooo(2)[of r c'], goal_cases)
+    case 1
+    then show ?case using s by auto
+  next
+    case (2 p' \<beta> c'')
+    hence re: "\<alpha>' < aux\<^sub>c r (c\<^sub>1' ; p') <\<^sub>c aux\<^sub>\<alpha> r \<beta>" using ooo(3) s by auto
+    then obtain \<beta>' where b: "\<beta>' < c\<^sub>1' ; p' <\<^sub>c \<beta>" using aux_re by blast
+
+    show ?case 
+      apply (rule ooo(5)[of "c\<^sub>1' ; p'" \<beta> "c\<^sub>1' ; c''"])
+      using s 2 b apply auto
+      apply (rule execute.ooo[of _ _ _ _ \<beta>'], simp)
+      by auto
+  qed 
+next
+  case (par1 c\<^sub>1 r' \<alpha> c\<^sub>1' c\<^sub>2)
+  then show ?case apply auto by force
+next
+  case (par2 c\<^sub>2 r' \<alpha> c\<^sub>2' c\<^sub>1)
+  then show ?case apply auto by force
+qed *)
+
+*)
+
+(* next
+  case (aux R G P c Q r')
+  thus ?case sorry then obtain c'' p' \<beta> where a: "c \<mapsto>[p',\<beta>] c''" "aux\<^sub>c r' c'' = c'" "\<alpha> = aux\<^sub>\<alpha> r' \<beta>" "r = aux\<^sub>c r' p'"
+    apply (elim aux_execE) by blast
+  then obtain P' M where p: "P \<subseteq> P'" "R,G \<turnstile>\<^sub>A P' {\<beta>\<llangle>p'\<rrangle>} M" "R,G \<turnstile> M {c''} Q"
+    using aux(2)[OF a(1)] by blast
+  have "aux\<^sub>P r' P \<subseteq> aux\<^sub>P r' P'" using p by (simp add: aux\<^sub>P_mono)
+  moreover have "aux\<^sub>R r' R,aux\<^sub>G r' G \<turnstile> aux\<^sub>P r' M {c'} aux\<^sub>P r' Q" using p  a(2) by blast
+  moreover have "aux\<^sub>R r' R,aux\<^sub>G r' G \<turnstile>\<^sub>A aux\<^sub>P r' P' {\<alpha>\<llangle>r\<rrangle>} aux\<^sub>P r' M"
+    using p(2) unfolding a by simp blast
+  ultimately show ?case by blast*)
+
+end
