Transition_Rules.thy
@@ -1,0 +1,212 @@
+theory Transition_Rules
+  imports Rules
+begin
+
+context rules
+begin
+
+text \<open>
+A series of lemmas that demonstrate the logic's rules are preserved across the semantic steps and
+ensure any executed behaviours conform to the desired specification.
+\<close>
+
+section \<open>Reordering Rules\<close> 
+
+text \<open>
+  Reorder the judgements of two reorderable instructions given a suitable interference property.
+  The precondition P and postcondition Q are preserved.
+\<close>
+lemma reorder_action:
+  assumes "R,G \<turnstile>\<^sub>A P {\<beta>} M" "R,G \<turnstile>\<^sub>A M {\<alpha>} Q" "inter\<^sub>\<alpha> R G \<beta> \<alpha>"
+  obtains M' where "R,G \<turnstile>\<^sub>A P {\<alpha>\<langle>tag \<beta>\<rangle>} M'" "R,G \<turnstile>\<^sub>A M' {\<beta>} Q"
+proof -
+  \<comment> \<open>Nominate the strongest-postcondition of \<alpha> from P as the state between \<alpha> and \<beta>\<close>
+  let ?M="{m. \<exists>m' m''. m' \<in> P \<and> (m',m'') \<in> beh (\<alpha>\<langle>tag \<beta>\<rangle>) \<and> (m'',m) \<in> R\<^sup>*}"
+
+  \<comment> \<open>Establish stability for P, Q and the new intermediate state, in addition to guarantees\<close>
+  have stablePQ: "stable R P" "stable R Q" "guar\<^sub>\<alpha> \<alpha> G" "guar\<^sub>\<alpha> \<beta> G"
+    using assms(1,2) by (auto simp: atomic_rule_def)
+  have stableM: "stable R ?M" unfolding stable_def by force
+
+  \<comment> \<open>Extract order independence properties\<close> 
+  have ref: "Env R ; Basic \<beta> ; Env R ; Basic \<alpha> \<sqsubseteq> Env R ; Basic \<alpha>\<langle>tag \<beta>\<rangle> ; Env R ; Basic \<beta>"
+    using assms(3) by (auto simp: inter\<^sub>\<alpha>_def)
+  have g: "guar\<^sub>\<alpha> \<alpha>\<langle>tag \<beta>\<rangle> G" using assms(3) by (auto simp: inter\<^sub>\<alpha>_def)
+
+  \<comment> \<open>Show transition from P to Q is independent of order\<close>
+  have p: "P \<subseteq> wp\<^sub>\<alpha> \<beta> M" "M \<subseteq> wp\<^sub>\<alpha> \<alpha> Q" "M \<subseteq> wp\<^sub>e R M" "P \<subseteq> wp\<^sub>e R P" "Q \<subseteq> wp\<^sub>e R Q"
+    using assms(1,2)  unfolding atomic_rule_def by (auto intro!: stable_wpI)
+  hence "P \<subseteq> wp\<^sub>e R (wp\<^sub>\<alpha> \<beta> (wp\<^sub>e R (wp\<^sub>\<alpha> \<alpha> Q)))" unfolding wp_def by blast
+  hence exec: "P \<subseteq> wp\<^sub>e R (wp\<^sub>\<alpha> \<alpha>\<langle>tag \<beta>\<rangle> (wp\<^sub>e R (wp\<^sub>\<alpha> \<beta> Q)))" using ref by (auto simp: refine_def)
+  hence vc: "P \<subseteq> vc \<alpha>\<langle>tag \<beta>\<rangle>" by (auto simp: wp_def)
+
+  \<comment> \<open>Establish the late judgement over \<beta>\<close>
+  have "R,G \<turnstile>\<^sub>A ?M {\<beta>} Q" 
+  proof (unfold atomic_rule_def, intro conjI Int_greatest)
+    show "?M \<subseteq> wp\<^sub>\<alpha> \<beta> Q" using exec unfolding wp_def by fast
+  qed (insert stablePQ stableM, auto)
+
+  \<comment> \<open>Establish the early judgement over the new \<alpha>\<close>
+  moreover have "R,G \<turnstile>\<^sub>A P {\<alpha>\<langle>tag \<beta>\<rangle>} ?M"
+  proof (unfold atomic_rule_def, intro conjI Int_greatest)
+    show "P \<subseteq> wp\<^sub>\<alpha> \<alpha>\<langle>tag \<beta>\<rangle> ?M" using vc unfolding wp_def wf_def by fast
+  qed (insert stablePQ stableM g, auto)
+
+  ultimately show ?thesis using that by blast
+qed
+
+text \<open>
+  Reorder the judgements of a reorderable instruction \<alpha> and program c, given a suitable 
+  interference property.
+\<close>
+lemma reorder_prog:
+  assumes "R,G \<turnstile> P {c} M" "R,G \<turnstile>\<^sub>A M {\<alpha>} Q" "inter\<^sub>c R G c \<alpha>"
+  obtains M' P' where "P \<subseteq> P'" "R,G \<turnstile>\<^sub>A P' {\<alpha>\<llangle>c\<rrangle>} M'" "R,G \<turnstile> M' {c} Q"
+  using assms
+proof (induct c arbitrary: R G P M Q \<alpha>)
+  case Nil
+  hence "P \<subseteq> M" by blast
+  then show ?case using Nil by (auto simp: atomic_rule_def)
+next
+  case (Basic \<beta>)
+  obtain P' N' where \<beta>: "P \<subseteq> P'" "R,G \<turnstile>\<^sub>A P' {\<beta>} N'" "N' \<subseteq> M" using Basic by auto
+  have m': "R,G \<turnstile>\<^sub>A N' {\<alpha>} Q"
+    using atomic_pre[OF Basic(3)] \<beta>(2,3) Basic(3) by (auto simp: atomic_rule_def)
+  obtain M' where m'': "R,G \<turnstile>\<^sub>A P' {\<alpha>\<langle>tag \<beta>\<rangle>} M'" "R,G \<turnstile>\<^sub>A M' {\<beta>} Q"
+    using reorder_action[OF \<beta>(2) m'(1)] Basic by auto
+  have "R,G \<turnstile> M' {Basic \<beta>} Q" by (rule rules.basic[OF m''(2)])
+  then show ?case using Basic(1) \<beta>(1) m''(1) by auto
+next
+  case (Seq c\<^sub>1 c\<^sub>2)
+  obtain M' where m: "R,G \<turnstile> P {c\<^sub>1} M'" "R,G \<turnstile> M' {c\<^sub>2} M" using Seq(4) by fast
+  have i: "inter\<^sub>c R G c\<^sub>1 \<alpha>\<llangle>c\<^sub>2\<rrangle>" "inter\<^sub>c R G c\<^sub>2 \<alpha>" using Seq by auto
+  show ?case
+  proof (rule Seq(2)[OF _ m(2) Seq(5) i(2)], goal_cases outer)
+    case (outer P' N')
+    hence c1: "R,G \<turnstile> P {c\<^sub>1} P'" using m(1) conseq by auto
+    show ?case 
+    proof (rule Seq(1)[OF _ c1 outer(2) i(1)], goal_cases inner)
+      case (inner P'' M'')
+      then show ?case using Seq(3) outer by auto
+    qed
+  qed
+next
+  case (Ord c\<^sub>1 c\<^sub>2)
+  obtain M' where m: "R,G \<turnstile> P {c\<^sub>1} M'" "R,G \<turnstile> M' {c\<^sub>2} M" using Ord(4) by fast
+  have i: "inter\<^sub>c R G c\<^sub>1 \<alpha>\<llangle>c\<^sub>2\<rrangle>" "inter\<^sub>c R G c\<^sub>2 \<alpha>" using Ord by auto
+  show ?case
+  proof (rule Ord(2)[OF _ m(2) Ord(5) i(2)], goal_cases outer)
+    case (outer P' N')
+    hence c1: "R,G \<turnstile> P {c\<^sub>1} P'" using m(1) conseq by auto
+    show ?case 
+    proof (rule Ord(1)[OF _ c1 outer(2) i(1)], goal_cases inner)
+      case (inner P'' M'')
+      then show ?case using Ord(3) outer by auto
+    qed
+  qed
+qed auto
+
+section \<open>Transition Rules\<close>
+
+text \<open>Judgements are preserved across silent steps\<close>
+lemma rewrite_ruleI [intro]:
+  assumes "R,G \<turnstile> P {c} Q"
+  assumes "c \<leadsto> c'"
+  shows "R,G \<turnstile> P {c'} Q"
+  using assms
+proof (induct arbitrary: c' rule: rules.induct)
+  case (seq R G P c\<^sub>1 Q c\<^sub>2 M)
+  thus ?case by (cases rule: silentE, auto) blast+
+next
+  case (ord R G P c\<^sub>1 Q c\<^sub>2 M)
+  thus ?case by (cases rule: silentE, auto) blast+
+qed (cases rule: silentE, auto)+
+
+text \<open>Judgements are preserved across thread-local execution steps\<close>
+lemma lexecute_ruleI [intro]:
+  assumes "R,G \<turnstile> P {c} Q" "c \<mapsto>[r,\<alpha>] c'"  "inter\<^sub>c R G r \<alpha>"
+  shows "\<exists>P' M. P \<subseteq> P' \<and> R,G \<turnstile>\<^sub>A P' {\<alpha>\<llangle>r\<rrangle>} M \<and> R,G \<turnstile> M {c'} Q"
+  using assms(2,1,3)
+proof (induct arbitrary: P R G Q)
+  case (act \<alpha>)
+  then show ?case by clarsimp (meson atomic_rule_def nil rules.conseq order_refl)
+next
+  case (ino c\<^sub>1 c \<alpha>' c\<^sub>1' c\<^sub>2)
+  then obtain M' where m: "R,G \<turnstile> P {c\<^sub>1} M'" "R,G \<turnstile> M' {c\<^sub>2} Q" by auto
+  then show ?case using ino(2)[OF m(1) ino(4)] m(2) by blast
+next
+  case (ooo c\<^sub>2 c \<alpha> c\<^sub>2' \<alpha>' c\<^sub>1)
+  obtain M' where m: "R,G \<turnstile> P {c\<^sub>1} M'" "R,G \<turnstile> M' {c\<^sub>2} Q" using ooo(4) by blast
+  have i: "inter\<^sub>c R G c\<^sub>1 (\<alpha>\<llangle>c\<rrangle>)" "inter\<^sub>c R G c \<alpha>" using ooo by auto
+  obtain P' M where m': "M' \<subseteq> P'" "R,G \<turnstile>\<^sub>A P' {\<alpha>\<llangle>c\<rrangle>} M" "R,G \<turnstile> M {c\<^sub>2'} Q"
+    using ooo(2)[OF m(2) i(2)] by blast
+  hence m'': "R,G \<turnstile> P {c\<^sub>1} P'" using m(1) by blast
+  then show ?case using reorder_prog[OF m'' m'(2)] i(1) m'(3) by simp (metis rules.seq)
+next
+  case (ord c\<^sub>1 c \<alpha> c\<^sub>1' c\<^sub>2)
+  obtain M' where m: "R,G \<turnstile> P {c\<^sub>1} M'" "R,G \<turnstile> M' {c\<^sub>2} Q" using ord by fast
+  then show ?case using ord(2)[OF m(1) ord(4)] m(2) by blast
+qed
+
+text \<open>Judgements are preserved across global execution steps\<close>
+lemma gexecute_ruleI [intro]:
+  assumes "R,G \<turnstile> P {c} Q"
+  assumes "c \<mapsto>[g] c'"
+  shows "\<exists>M v. P \<subseteq> wp v g M \<and> guar v g G \<and> R,G \<turnstile> M {c'} Q"
+  using assms
+proof (induct arbitrary: g c' rule: rules.induct)
+  case (par R\<^sub>1 G\<^sub>1 P\<^sub>1 c\<^sub>1 Q\<^sub>1 R\<^sub>2 G\<^sub>2 P\<^sub>2 c\<^sub>2 Q\<^sub>2)
+  show ?case using par(7)
+  proof cases
+    case (par1 c\<^sub>1')
+    obtain M\<^sub>2 where m2: "P\<^sub>2 \<subseteq> M\<^sub>2" "stable R\<^sub>2 M\<^sub>2" "R\<^sub>2,G\<^sub>2 \<turnstile> M\<^sub>2 {c\<^sub>2} Q\<^sub>2" using par
+      by (meson stable_preE)
+    obtain M\<^sub>1 v where m1: "P\<^sub>1 \<subseteq> wp v g M\<^sub>1" "guar v g G\<^sub>1" "R\<^sub>1,G\<^sub>1 \<turnstile> M\<^sub>1 {c\<^sub>1'} Q\<^sub>1" 
+      using par1 par(2)[OF par1(2)] by blast
+    hence "R\<^sub>1 \<inter> R\<^sub>2,G\<^sub>1 \<union> G\<^sub>2 \<turnstile> M\<^sub>1 \<inter> M\<^sub>2 {c'} Q\<^sub>1 \<inter> Q\<^sub>2" using par1 m2 par by blast
+    moreover have "P\<^sub>1 \<inter> P\<^sub>2 \<subseteq> wp v g (M\<^sub>1 \<inter> M\<^sub>2)" 
+      using m1(1,2) m2(1,2) par.hyps(6) unfolding guar_def wp_def stable_def
+      by auto blast
+    ultimately show ?thesis using m1(2) unfolding guar_def by blast
+  next
+    case (par2 c\<^sub>2')
+    obtain M\<^sub>1 where m1: "P\<^sub>1 \<subseteq> M\<^sub>1" "stable R\<^sub>1 M\<^sub>1" "R\<^sub>1,G\<^sub>1 \<turnstile> M\<^sub>1 {c\<^sub>1} Q\<^sub>1" using par
+      by (meson stable_preE)
+    obtain M\<^sub>2 v where m2: "P\<^sub>2 \<subseteq> wp v g M\<^sub>2" "guar v g G\<^sub>2" "R\<^sub>2,G\<^sub>2 \<turnstile> M\<^sub>2 {c\<^sub>2'} Q\<^sub>2" 
+      using par2 par(4)[OF par2(2)] by blast
+    hence "R\<^sub>1 \<inter> R\<^sub>2,G\<^sub>1 \<union> G\<^sub>2 \<turnstile> M\<^sub>1 \<inter> M\<^sub>2 {c'} Q\<^sub>1 \<inter> Q\<^sub>2" using par2 m1 par by blast
+    moreover have "P\<^sub>1 \<inter> P\<^sub>2 \<subseteq> wp v g (M\<^sub>1 \<inter> M\<^sub>2)" 
+      using m1(1,2) m2(1,2) par.hyps(5) unfolding guar_def wp_def stable_def
+      by auto blast
+    ultimately show ?thesis using m2(2) unfolding guar_def by blast
+  qed 
+next
+  case (conseq R G P c Q P' R' G' Q')
+  thus ?case by (smt Un_iff guar_def rules.conseq subset_iff)
+next
+  case (inv R G P c Q R' M')
+  then obtain M v where p: "P \<subseteq> wp v g M" "guar v g G" "R,G \<turnstile> M {c'} Q" by metis
+  hence "P \<inter> M' \<subseteq> wp v g (M \<inter> M')" using inv(3,4) by (auto simp: stable_def guar_def wp_def) blast
+  thus ?case using rules.inv p(2,3) inv(3,4) by blast
+next       
+  case (thread R G P c Q op l)
+  \<comment> \<open>Convert the global execution step into a local execution step\<close>
+  obtain r \<alpha> c\<^sub>t l' where thr: "g = thr2glb op l l' (beh \<alpha>\<llangle>r\<rrangle>)" "c' = Thread l' op c\<^sub>t" "c \<mapsto>[r,\<alpha>] c\<^sub>t"
+    using thread by auto
+  \<comment> \<open>As this is the thread rule case, we have the interference-freedom property\<close>
+  \<comment> \<open>Split this interference-freedom property based on the local execution step\<close>
+  hence i: "inter R G c\<^sub>t" "inter\<^sub>c R G r \<alpha>" using thread indep_stepI by auto
+  \<comment> \<open>Use the lexecute rule to extract the desired logic judgement and properties\<close>
+  then obtain M where p: "P \<subseteq> wp\<^sub>\<alpha> \<alpha>\<llangle>r\<rrangle> M" "guar\<^sub>\<alpha> \<alpha>\<llangle>r\<rrangle> G" "R,G \<turnstile> M {c\<^sub>t} Q" 
+    using lexecute_ruleI[OF thread(1) thr(3)] by (auto simp: atomic_rule_def)
+  \<comment> \<open>Demonstrate these properties are preserved when the local state is obfuscated\<close>
+  hence "thr\<^sub>P op l P \<subseteq> wp (thr\<^sub>P op l (vc \<alpha>\<llangle>r\<rrangle>)) g (thr\<^sub>P op l' M)"
+    using thr_wp thr(1) by fast
+  moreover have "guar (thr\<^sub>P op l (vc \<alpha>\<llangle>r\<rrangle>)) g (thr\<^sub>G op G)"
+    using p(2) thr_guar thr(1) by fast
+  ultimately show ?case using p i unfolding thr(2) by blast
+qed auto
+
+end
+
+end
